completing Imp

Frap/Imp.lean
@@ -1,7 +1,15 @@
 import Lean.Data.HashMap
 
 /-
+# Towards an imperative programming language
+
+We start formal reasoning about programs (for real) by introducing a programming language into Lean.
+We begin with a language that everyone should be familiar with, in the _imperative language_ paradigm.
+Constructs in an imperative language features statements and commands, such as assignments, conditionals, and loops.
+
 ## Arithmetic and boolean expressions
+
+We begin with the definition of arithmetic and boolean expressions, defined inductively.
 
 ### Syntax
 -/
@@ -29,6 +37,9 @@ open BExp
 
 /-
 ### Evaluation
+
+We evaluate arithmetic and boolean expressions recursively.
+(Note: we can write subscripts such as `a₁` by typing `a\1`.)
 -/
 
 def aeval (a : AExp) : Nat :=
@@ -49,10 +60,11 @@ def beval (b : BExp) : Bool :=
   | b_and b₁ b₂ => and (beval b₁) (beval b₂)
   | b_or b₁ b₂ => or (beval b₁) (beval b₂)
 
-#eval beval (b_le (a_num 7) (a_num 5))
-
 /-
 ### Optimization
+
+Right away, we can introduce some optimization prior to evaluation so that our expression tree is as compact as possible.
+Here, we will optimize additions with zero on the left-hand side, and prove that the optimization preserves the meaning of the expression.
 -/
 
 def optimize_0plus (a : AExp) : AExp :=
@@ -92,21 +104,30 @@ theorem optimize_0plus_sound (a : AExp)
       rw [iha₁, iha₂]
 
 /-
-exercise (3-star)
-Since the `optimize_0plus` transformation doesn't change the value of `AExp`s, we should be able to apply it to all the `AExp`s that appear in a `BExp` without changing the `BExp`'s value.
-Write a function that performs this transformation on `BExp`s and prove it is sound.
-Use tactic combinators to make the proof as short and elegant as possible.
+exercise (2-star)
+Define an optimizations for additions with zero on the right-hand side, and prove that the optimization preserves the meaning of the expression.
 -/
 
-def optimize_0plus_b (b : BExp) : BExp :=
+def optimize_plus0 (a : AExp) : AExp :=
   sorry
 
-theorem optimize_0plus_b_sound (b : BExp)
-    : beval (optimize_0plus_b b) = beval b := by
+example : optimize_plus0
+      (a_plus (a_num 2)
+              (a_plus (a_plus (a_num 1) (a_num 0))
+                      (a_num 0)))
+    = a_plus (a_num 2) (a_num 1) := by
+  sorry
+
+theorem optimize_plus0_sound (a : AExp)
+    : aeval (optimize_plus0 a) = aeval a := by
   sorry
 
 /-
 ## Evaluation as a relation
+
+Previously, we defined a recursive function to compute the result of an expression.
+While that approach usually works most of the time, it can make proofs less automatable and more convoluted.
+An alternative is to define an inductive relation between expressions and their values.
 -/
 
 inductive AEvalR : AExp → Nat → Prop :=
@@ -118,10 +139,14 @@ inductive AEvalR : AExp → Nat → Prop :=
   | e_a_mult (a₁ a₂ : AExp) (n₁ n₂ : Nat) :
       AEvalR a₁ n₁ → AEvalR a₂ n₂ → AEvalR (a_mult a₁ a₂) (n₁ * n₂)
 
+/-
+We can introduce a notation that makes expressions look more natural in Lean code.
+We'll write `e ==> n` to mean that arithmetic expression `e` evaluates to value `n`.
+-/
 infix:90 " ==> " => AEvalR
 
 /-
-It is straightforward to prove that the relational and functional definitions of evaluation agree.
+It is (almost) straightforward to prove that the relational and functional definitions of evaluation agree.
 -/
 
 example (a : AExp) (n : Nat)
@@ -136,6 +161,16 @@ example (a : AExp) (n : Nat)
       sorry
     | _ => sorry
 
+/-
+In the proof above, we see that our induction is stuck, because the result of every `AExp` evaluation is `n`.
+This is because when we perform induction, we have already introduced and fixed `n` as a parameter of the theorem.
+As a result, the induction hypotheses become `aeval a₁ = n → a₁ ==> n` and `aeval a₂ = n → a₂ ==> n`.
+But this statement ought to work for any value of `n`, so our induction hypotheses should be `∀ (n : Nat), aeval a₁ = n → a₁ ==> n` and `∀ (n : Nat), aeval a₂ = n → a₂ ==> n`.
+We can reintroduce the universal quantifier by using a variant of the `induction` tactic that _generalizes_ over some variables before applying the induction but then introduces them in each goal.
+
+Now, our proof goes through.
+-/
+
 theorem aeval_iff_AEvalR (a : AExp) (n : Nat)
     : a ==> n ↔ aeval a = n := by
   constructor
@@ -146,24 +181,17 @@ theorem aeval_iff_AEvalR (a : AExp) (n : Nat)
     | a_num n' => constructor
     | _ => rw [← h]; constructor <;> assumption
 
-/-
-exercise (3-star)
-Write a relation `BEvalR` in the same style as `AEvalR`, and prove that it is equivalent to `beval`.
--/
-
-inductive BEvalR : BExp → Bool → Prop :=
-  /- **fill in here** -/
-
-infix:90 " ==>b " => BEvalR
-
-theorem beval_iff_BEvalR b bv
-    : b ==>b bv ↔ beval v = bv := by
-  sorry
-
 end Hidden.AExp
 
 /-
 ### Computational vs relational definitions
+
+In certain situations, relational definitions of evaluation works much better than computation ones.
+
+For example, suppose we want to add division as another possible expression.
+How do we deal with division by zero?
+What should be the result returned from `aeval` function?
+But in `AEvalR`, we can easily specify a precondition on when results will be available.
 -/
 
 namespace AEvalR_division
@@ -191,6 +219,11 @@ inductive AEvalR : AExp → Nat → Prop :=
 
 end AEvalR_division
 
+/-
+Or when we want to add a random number generator...
+Here, we are saying what results are _possible_, without specifying any particular probability distributions for the results.
+-/
+
 namespace AEvalR_extended
 
 inductive AExp where
@@ -214,13 +247,18 @@ inductive AEvalR : AExp → Nat → Prop :=
 
 end AEvalR_extended
 
+namespace Imp
+
 /-
 ## Expressions with variables
+
+In a typical imperative language, expressions may contain variables.
+For simplicity (for now), we'll assume that all variables are global and that they only hold numbers.
 -/
 
 inductive AExp where
   | a_num : Nat → AExp
-  | a_id : String → AExp  -- new
+  | a_id : String → AExp  -- new case
   | a_plus : AExp → AExp → AExp
   | a_minus : AExp → AExp → AExp
   | a_mult : AExp → AExp → AExp
@@ -243,48 +281,118 @@ inductive BExp where
 open AExp
 open BExp
 
-declare_syntax_cat expr
+/-
+Here, we declare a set of macros that will naturalize the appearance of expressions, so we have an easier time staring at them.
 
-syntax num : expr
-syntax str : expr
-syntax:60 expr:60 "+" expr:61 : expr
-syntax:60 expr:60 "-" expr:61 : expr
-syntax:70 expr:70 "*" expr:71 : expr
-syntax:50 expr:50 "=" expr:50 : expr
-syntax:50 expr:50 "!=" expr:50 : expr
-syntax:50 expr:50 "<=" expr:50 : expr
-syntax:40 "!" expr:40 : expr
-syntax:30 expr:30 "&&" expr:31 : expr
-syntax:30 expr:30 "||" expr:31 : expr
-syntax "True" : expr
-syntax "False" : expr
-syntax "(" expr ")" : expr
+This is a somewhat advanced feature of Lean, so you don't need to understand it entirely yet, but it can be helpful when doing a larger project, as this will save you time writing down Lean terms.
+-/
 
-syntax "<{" expr "}>" : term
+declare_syntax_cat imp
+
+syntax num : imp
+syntax str : imp
+syntax:60 imp:60 "+" imp:61 : imp
+syntax:60 imp:60 "-" imp:61 : imp
+syntax:70 imp:70 "*" imp:71 : imp
+syntax:50 imp:50 "=" imp:50 : imp
+syntax:50 imp:50 "!=" imp:50 : imp
+syntax:50 imp:50 "<=" imp:50 : imp
+syntax:40 "!" imp:40 : imp
+syntax:30 imp:30 "&&" imp:31 : imp
+syntax:30 imp:30 "||" imp:31 : imp
+syntax "True" : imp
+syntax "False" : imp
+syntax "(" imp ")" : imp
+syntax "<{" imp "}>" : term
+syntax ident : imp
+syntax "<[" term "]>" : imp
+
 macro_rules
-  | `(<{$n:num}>) => `(a_num $n)
-  | `(<{$s:str}>) => `(a_id $s)
-  | `(<{$x + $y}>) => `(a_plus <{$x}> <{$y}>)
-  | `(<{$x - $y}>) => `(a_minus <{$x}> <{$y}>)
-  | `(<{$x * $y}>) => `(a_mult <{$x}> <{$y}>)
-  | `(<{True}>) => `(b_true)
-  | `(<{False}>) => `(b_false)
-  | `(<{$x = $y}>) => `(b_eq <{$x}> <{$y}>)
-  | `(<{$x != $y}>) => `(b_neq <{$x}> <{$y}>)
-  | `(<{$x <= $y}>) => `(b_le <{$x}> <{$y}>)
-  | `(<{!$x}>) => `(b_not <{$x}>)
-  | `(<{$x && $y}>) => `(b_and <{$x}> <{$y}>)
-  | `(<{$x || $y}>) => `(b_or <{$x}> <{$y}>)
+  | `(term|<{$x}>) => `(imp|$x)
+  | `(imp|$n:num) => `(a_num $n)
+  | `(imp|$s:str) => `(a_id $s)
+  | `(imp|$x + $y) => `(a_plus <{$x}> <{$y}>)
+  | `(imp|$x - $y) => `(a_minus <{$x}> <{$y}>)
+  | `(imp|$x * $y) => `(a_mult <{$x}> <{$y}>)
+  | `(imp|True) => `(b_true)
+  | `(imp|False) => `(b_false)
+  | `(imp|$x = $y) => `(b_eq <{$x}> <{$y}>)
+  | `(imp|$x != $y) => `(b_neq <{$x}> <{$y}>)
+  | `(imp|$x <= $y) => `(b_le <{$x}> <{$y}>)
+  | `(imp|!$x) => `(b_not <{$x}>)
+  | `(imp|$x && $y) => `(b_and <{$x}> <{$y}>)
+  | `(imp|$x || $y) => `(b_or <{$x}> <{$y}>)
+  | `(imp|($x)) => `(<{$x}>)
+  | `(imp|$x:ident) => `(a_id $(Lean.quote (toString x.getId)))
+  | `(imp|<[$t:term]>) => pure t
 
-open Lean
-open Lean.HashMap
+/-
+### States
 
-abbrev State := HashMap String Nat
+To evaluate expressions with variables, we need a place to look up the value of a variable.
+We will use an _association list_ for this purpose, with 0 as the default value.
+Of course, in real systems, we would use a more efficient data structure, which we can _prove_ that it works the same way, i.e., we can interchange data structures for states without affecting the correctness of the evaluation.
+-/
+
+abbrev State := List (String × Nat)
+
+open List
+
+def empty : State := nil
+
+def insert' (st : State) (k : String) (v : Nat) : State :=
+  match st with
+  | nil => [(k, v)]
+  | cons (k', v') st' =>
+    if k == k' then cons (k, v) st'
+    else cons (k', v') (insert' st' k v)
+
+def lookup' (st : State) (k : String) : Nat :=
+  match st with
+  | nil => 0
+  | cons (k', v') st' =>
+    if k == k' then v' else lookup' st' k
+
+/-
+We can prove properties about our association lists as states.
+-/
+
+theorem map_lookup_insert_eq st (x : String) (v : Nat)
+    : lookup' (insert' st x v) x = v := by
+  induction st with
+  | nil => simp [lookup']
+  | cons p st' ih =>
+    obtain ⟨k', v'⟩ := p
+    unfold insert'
+    split
+    . simp [lookup']
+    . simp [lookup', *]
+
+theorem map_lookup_insert_neq st (x x' : String) (v : Nat)
+    : x' ≠ x
+      → lookup' (insert' st x v) x' = lookup' st x' := by
+  intro hneq
+  induction st with
+  | nil => simp [lookup', *]
+  | cons p st' ih =>
+    obtain ⟨k', v'⟩ := p
+    unfold insert'
+    split
+    . simp [lookup', *] at *
+      have h: x' ≠ k' := by
+        intro hneq'; apply hneq
+        rw [hneq']; apply Eq.symm; assumption
+      simp [h]
+    . simp [lookup', *]
+
+/-
+The evaluation functions now require a state as an argument.
+-/
 
 def aeval (st : State) (a : AExp) : Nat :=
   match a with
   | a_num n => n
-  | a_id x => find! st x
+  | a_id x => lookup' st x
   | a_plus a₁ a₂ => (aeval st a₁) + (aeval st a₂)
   | a_minus a₁ a₂ => (aeval st a₁) - (aeval st a₂)
   | a_mult a₁ a₂ => (aeval st a₁) * (aeval st a₂)
@@ -300,17 +408,59 @@ def beval (st : State) (b : BExp) : Bool :=
   | b_and b₁ b₂ => and (beval st b₁) (beval st b₂)
   | b_or b₁ b₂ => or (beval st b₁) (beval st b₂)
 
-theorem map_lookup_insert (x : String) (v : Nat)
-    : find! (insert empty x v) x = v := by
-  sorry
+/-
+We can try evaluating some expressions under given states.
+-/
 
-example : aeval (insert empty x 5)
-    (a_plus (a_num 3) (a_mult (a_id x) (a_num 2)))
+example : aeval (insert' empty x 5)
+    <{3 + x * 2}>
+    -- (a_plus (a_num 3) (a_mult (a_id x) (a_num 2)))
     = 13 := by
-  simp [aeval, map_lookup_insert]
+  simp [aeval, map_lookup_insert_eq]
+
+example : aeval (insert' (insert' empty y 4) x 5)
+    <{z + x * y}>
+    = 20 := by
+  simp [x, y, aeval, lookup', insert', map_lookup_insert_eq]
+
+example : beval (insert' empty x 5)
+    <{ True && !(x <= 4) }>
+    = true := by
+  simp [x, beval, insert', aeval, lookup']
+
+/-
+We can define evaluation as a relation, like before.
+But we need to talk about state in our relation.
+-/
+
+inductive AEvalR : State → AExp → Nat → Prop :=
+  | e_a_num (st : State) (n : Nat) : AEvalR st (a_num n) n
+  | e_a_id (st : State) (x : String) (n : Nat) :
+      lookup' st x = n → AEvalR st (a_id x) n
+  | e_a_plus (st : State) (a₁ a₂ : AExp) (n₁ n₂ : Nat) :
+      AEvalR st a₁ n₁ → AEvalR st a₂ n₂ → AEvalR st (a_plus a₁ a₂) (n₁ + n₂)
+  | e_a_minus (st : State) (a₁ a₂ : AExp) (n₁ n₂ : Nat) :
+      AEvalR st a₁ n₁ → AEvalR st a₂ n₂ → AEvalR st (a_minus a₁ a₂) (n₁ - n₂)
+  | e_a_mult (st : State) (a₁ a₂ : AExp) (n₁ n₂ : Nat) :
+      AEvalR st a₁ n₁ → AEvalR st a₂ n₂ → AEvalR st (a_mult a₁ a₂) (n₁ * n₂)
+
+/-
+Our proof of equivalence of the definitions only needs a little bit of tweaks.
+-/
+
+/-
+exercise (2-star)
+Prove that, on the augmented version of arithmetic expressions, the functional and relational definitions are equivalent.
+-/
+
+theorem aeval_iff_AEvalR (st : State) (a : AExp) (n : Nat)
+    : AEvalR st a n ↔ aeval st a = n := by
+  sorry
 
 /-
 ## Behavioral equivalence
+
+To talk about the correctness of program transformations, we need to be able to say when two expressions are _behaviorally equivalent_, i.e., they evaluate to the same result in every state.
 -/
 
 def aequiv (a₁ a₂ : AExp) : Prop :=
@@ -320,17 +470,24 @@ def bequiv (b₁ b₂ : BExp) : Prop :=
   ∀ (st : State), beval st b₁ = beval st b₂
 
 theorem aequiv_example
-    : aequiv <{"x" - "x"}> <{0}> := by
+    : aequiv <{x - x}> <{0}> := by
   intro st
   simp [aeval]
 
 theorem bequiv_example
-    : bequiv <{"x" - "x" = 0}> <{True}> := by
+    : bequiv <{x - x = 0}> <{True}> := by
   intro st
   simp [beval, aeval]
 
 /-
 ## Commands
+
+We now introduce commands in our imperative language:
+* `skip`: do nothing
+* `x := a`: assignment to a variable
+* `c₁; c₂`: do `c₁`, then `c₂` (sequencing operation)
+* `if b then c₁ else c₂`: conditional statement
+* `while b do c end`: loop
 -/
 
 inductive Com :=
@@ -340,8 +497,62 @@ inductive Com :=
   | c_if : BExp → Com → Com → Com
   | c_while : BExp → Com → Com
 
+open Com
+
+syntax "skip" : imp
+syntax:20 imp:20 ":=" imp:21 : imp
+syntax:20 imp:20 ";" imp:20 : imp
+syntax:20 "if" imp:20 "then" imp:20 "else" imp:20 : imp
+syntax:20 "while" imp:20 "do" imp:20 "end" : imp
+
+macro_rules
+  | `(imp|skip) => `(c_skip)
+  | `(imp|$x:str := $y) => `(c_asgn $x <{$y}>)
+  | `(imp|$x:ident := $y) => `(c_asgn $x <{$y}>)
+  | `(imp|$c1 ; $c2) => `(c_seq <{$c1}> <{$c2}>)
+  | `(imp|if $b then $c1 else $c2) => `(c_if <{$b}> <{$c1}> <{$c2}>)
+  | `(imp|while $b do $c end) => `(c_while <{$b}> <{$c}>)
+
+/-
+We can write some simple programs in our macro language, _without worrying about their meaning_ just yet.
+-/
+
+def factorial_in_lean4 : Com :=
+  <{ z := x;
+     y := 1;
+     while z != 0 do
+       y := y * z;
+       z := (z - 1)
+     end }>
+
+def plus2 : Com := <{ x := x + 2 }>
+
+def xTimesYInZ : Com := <{ z := x * y }>
+
+def subtract_slowly_body : Com :=
+  <{ z := z - 1;
+     x := x - 1 }>
+
+def subtract_slowly : Com :=
+  <{ while x != 0 do
+       <[subtract_slowly_body]>
+     end }>
+
+def subtract_3_from_5_slowly : Com :=
+  <{ x := 3;
+     z := 5;
+     <[subtract_slowly]> }>
+
+def loop : Com :=
+  <{ while True do
+       skip
+     end }>
+
 /-
 ## references
-* [](https://softwarefoundations.cis.upenn.edu/lf-current/Imp.html)
-* [](https://raw.githubusercontent.com/blanchette/logical_verification_2023/main/hitchhikers_guide.pdf)
+* [Software Foundations, Volume 1 Logical Foundations: Simple Imperative Programs](https://softwarefoundations.cis.upenn.edu/lf-current/Imp.html)
+* [Software Foundations, Volume 2 Programming Language Foundations: Program Equivalence](https://softwarefoundations.cis.upenn.edu/plf-current/Equiv.html)
+* [Lean Manual: Macro Overview](https://lean-lang.org/lean4/doc/macro_overview.html)
+* [Lean Manual: Arithmetic DSL](https://lean-lang.org/lean4/doc/metaprogramming-arith.html)
+* Anne Baanen, Alexander Bentkamp, Janmin Blanchette, Johannes Hölzl, Jannis Limperg. [The Hitchhiker's Guide to Logical Verification](https://raw.githubusercontent.com/blanchette/logical_verification_2023/main/hitchhikers_guide.pdf), version November 21, 2023.  Chapter 5.7.
 -/
