Frap/Exercises/Imp.lean
@@ -1,0 +1,57 @@
+-- imperative language exercises
+
+import Frap.Imp
+
+/-
+Here, we will work with the original version of arithmetic and boolean expressions (before adding identifiers).
+-/
+
+namespace Hidden.AExp
+
+open AExp
+open BExp
+
+/-
+exercise (1-star)
+Prove that the combination of the two optimizations involving zero still preserves the meaning of arithmetic expressions.
+You may use results from the lecture without proofs.
+-/
+
+def optimize_plus_with_0 (a : AExp) : AExp :=
+  optimize_plus0 (optimize_0plus a)
+
+theorem optimize_plus_with_0_sound (a : AExp)
+    : aeval (optimize_plus_with_0 a) = aeval a := by
+  sorry
+
+/-
+exercise (3-star)
+Since the `optimize_0plus` transformation doesn't change the value of `AExp`s, we should be able to apply it to all the `AExp`s that appear in a `BExp` without changing the `BExp`'s value.
+Write a function that performs this transformation on `BExp`s and prove it is sound.
+Use tactic combinators to make the proof as short and elegant as possible.
+-/
+
+def optimize_0plus_b (b : BExp) : BExp :=
+  sorry
+
+theorem optimize_0plus_b_sound (b : BExp)
+    : beval (optimize_0plus_b b) = beval b := by
+  sorry
+
+/-
+exercise (3-star)
+Write a relation `BEvalR` in the same style as `AEvalR`, and prove that it is equivalent to `beval`.
+-/
+
+inductive BEvalR : BExp → Bool → Prop :=
+  /- **fill in here** -/
+
+infix:90 " ==>b " => BEvalR
+
+open BEvalR
+
+theorem beval_iff_BEvalR b v
+    : b ==>b v ↔ beval b = v := by
+  sorry
+
+end Hidden.AExp
